Strata/Languages/Core/SMTEncoder.lean
@@ -286,7 +286,7 @@ partial def toSMTTerm (E : Env) (bvs : BoundVars) (e : LExpr CoreLParams.mono) (
         (Encoder.sanitizeSmtName b, s)
     let ctx := { ctx with bvCounter := ctx.bvCounter + 1 }
     -- Check for clashes with existing bvars, fvars in ctx, and fvars in body
-    let usedNames := bvs.map (·.1) ++ ctx.ufs.toList.map (·.id) ++ fvarNames.toList
+    let usedNames := Std.HashSet.ofList (bvs.map (·.1) ++ ctx.ufs.toList.map (·.id) ++ fvarNames.toList)
     let x := Strata.Name.findUnique baseName startSuffix usedNames
     let (ety, ctx) ← LMonoTy.toSMTType E ty ctx useArrayTheory
     let (trt, ctx) ← appToSMTTerm E ((x, ety) :: bvs) tr [] ctx useArrayTheory
